first succesful irisGS instance (prog is weird, though)

theories/progLog.v
@@ -1,7 +1,7 @@
 From iris.proofmode Require Import proofmode.
 From iris.base_logic Require Export invariants gen_heap.
 From iris.program_logic Require Export weakestpre ectx_lifting.
-From iris.algebra Require Import frac auth.
+From iris.algebra Require Import frac auth gmap excl.
 From ASMinCoq Require Export AsmGen.
 
 (* CMRΑ for memory *)
@@ -15,10 +15,209 @@ Class regG Σ := RegG {
   reg_gen_regG :: gen_heapGS Reg Word Σ; }.
 
 
+(* Stuff for the trace copied from Katamaran *)
+Class traceG (Trace : Type) Σ := TraceG {
+    trace_inG :: inG Σ (authR (optionUR (exclR (leibnizO Trace))));
+    trace_name : gname
+}.
+
+Definition tracePreΣ (Trace : Type) : gFunctors := #[GFunctor (authR (optionUR (exclR (leibnizO Trace))))].
+
+Class trace_preG (Trace : Type) Σ := {
+  trace_preG_inG :: inG Σ (authR (optionUR (exclR (leibnizO Trace))));
+}.
+
+#[export] Instance traceG_preG `{traceG T Σ} : trace_preG T Σ.
+Proof. constructor. typeclasses eauto. Defined.
+
+#[export] Instance subG_tracePreΣ {Σ T}:
+  subG (tracePreΣ T) Σ →
+  trace_preG T Σ.
+Proof. solve_inG. Qed.
+
+Section S.
+  Context `{!trace_preG T Σ}.
+  Context (γ : gname). (* To allow using different gnames *)
+
+  Definition tr_auth (t: T) : iProp Σ := own γ (● (Some (Excl (t: leibnizO T)))).
+  Definition tr_frag (t: T) : iProp Σ := own γ (◯ (Some (Excl (t: leibnizO T)))).
+
+  Lemma trace_full_frag_eq t t':
+    tr_auth t -∗ tr_frag t' -∗
+    ⌜ t = t' ⌝.
+  Proof.
+    iIntros "H1 H2".
+    iDestruct (own_valid_2 with "H1 H2") as %[Hi Hv]%auth_both_valid_discrete.
+    rewrite Excl_included in Hi.  apply leibniz_equiv in Hi. subst; auto.
+  Qed.
+
+  Lemma tr_frag_excl t t' :
+    tr_frag t -∗ tr_frag t' -∗ ⌜ False ⌝.
+  Proof.
+    iIntros "H1 H2". iDestruct (own_valid_2 with "H1 H2") as %Hv.
+    now apply excl_auth.excl_auth_frag_op_valid in Hv.
+  Qed.
+
+  Lemma trace_update t t' :
+    tr_auth t ∗ tr_frag t ==∗
+    tr_auth t' ∗ tr_frag t'.
+  Proof.
+    rewrite /tr_auth /tr_frag. rewrite -!own_op.
+    iApply own_update. apply auth_update.
+    apply option_local_update.
+    apply exclusive_local_update. constructor.
+  Qed.
+
+  (* For the moment, there is no need for a lemma stating that traces can only be appened to, but we could customize the RA to enforce this. *)
+
+  #[export] Instance tr_auth_Timeless t : Timeless (tr_auth t).
+  Proof.
+    intros. apply _.
+  Qed.
+
+  #[export] Instance tr_frag_Timeless t : Timeless (tr_frag t).
+  Proof.
+    intros. apply _.
+  Qed.
+End S.
+
+(* Stuff for the PC *)
+Class pcG Σ := PcG {
+    PC_inG :: inG Σ (authR (optionUR (exclR (leibnizO Word))));
+    PC_name : gname
+}.
+
+Definition PcPreΣ : gFunctors := #[GFunctor (authR (optionUR (exclR (leibnizO 
+Word))))].
+
+Class PC_preG Σ := {
+  PC_preG_inG :: inG Σ (authR (optionUR (exclR (leibnizO Word))));
+}.
+
+#[export] Instance PcG_preG `{pcG Σ} : PC_preG Σ.
+Proof. constructor. typeclasses eauto. Defined.
+
+#[export] Instance subG_PcPreΣ {Σ}:
+  subG PcPreΣ Σ →
+  PC_preG Σ.
+Proof. solve_inG. Qed.
+
+Section S.
+  Context `{!PC_preG Σ}.
+  Context (γ : gname). (* To allow using different gnames *)
+
+  Definition pc_auth (w : Word) : iProp Σ := own γ (● (Some (Excl (w : leibnizO Word)))).
+  Definition pc_frag (w : Word) : iProp Σ := own γ (◯ (Some (Excl (w : leibnizO Word)))).
+
+  Lemma pc_full_frag_eq t t':
+    pc_auth t -∗ pc_frag t' -∗
+    ⌜ t = t' ⌝.
+  Proof.
+    iIntros "H1 H2".
+    iDestruct (own_valid_2 with "H1 H2") as %[Hi Hv]%auth_both_valid_discrete.
+    rewrite Excl_included in Hi. apply leibniz_equiv in Hi. subst; auto.
+  Qed.
+
+  Lemma pc_frag_excl t t' :
+    pc_frag t -∗ pc_frag t' -∗ ⌜ False ⌝.
+  Proof.
+    iIntros "H1 H2". iDestruct (own_valid_2 with "H1 H2") as %Hv.
+    now apply excl_auth.excl_auth_frag_op_valid in Hv.
+  Qed.
+
+  Lemma pc_update t t' :
+    pc_auth t ∗ pc_frag t ==∗
+    pc_auth t' ∗ pc_frag t'.
+  Proof.
+    rewrite /pc_auth /pc_frag. rewrite -!own_op.
+    iApply own_update. apply auth_update.
+    apply option_local_update.
+    apply exclusive_local_update. constructor.
+  Qed.
+
+  (* For the moment, there is no need for a lemma stating that traces can only be appened to, but we could customize the RA to enforce this. *)
+
+  #[export] Instance pc_auth_Timeless t : Timeless (pc_auth t).
+  Proof.
+    intros. apply _.
+  Qed.
+
+  #[export] Instance pc_frag_Timeless t : Timeless (pc_frag t).
+  Proof.
+    intros. apply _.
+  Qed.
+End S.
+
+(* Stuff for the prog *)
+Class programG Σ := ProgramG {
+    Program_inG :: inG Σ (authR (optionUR (exclR (leibnizO program))));
+    Program_name : gname
+}.
+
+Definition ProgramPreΣ : gFunctors := #[GFunctor (authR (optionUR (exclR (leibnizO program))))].
+
+Class Program_preG Σ := {
+  Program_preG_inG :: inG Σ (authR (optionUR (exclR (leibnizO program))));
+}.
+
+#[export] Instance ProgramG_preG `{programG Σ} : Program_preG Σ.
+Proof. constructor. typeclasses eauto. Defined.
+
+#[export] Instance subG_ProgramPreΣ {Σ}:
+  subG ProgramPreΣ Σ →
+  Program_preG Σ.
+Proof. solve_inG. Qed.
+
+Section S.
+  Context `{!Program_preG Σ}.
+  Context (γ : gname). (* To allow using different gnames *)
+
+  Definition program_auth (p : program) : iProp Σ := own γ (● (Some (Excl (p : leibnizO program)))).
+  Definition program_frag (p : program) : iProp Σ := own γ (◯ (Some (Excl (p : leibnizO program)))).
+
+  Lemma program_full_frag_eq t t':
+    program_auth t -∗ program_frag t' -∗
+    ⌜ t = t' ⌝.
+  Proof.
+    iIntros "H1 H2".
+    iDestruct (own_valid_2 with "H1 H2") as %[Hi Hv]%auth_both_valid_discrete.
+    rewrite Excl_included in Hi. apply leibniz_equiv in Hi. subst; auto.
+  Qed.
+
+  Lemma program_frag_excl t t' :
+    program_frag t -∗ program_frag t' -∗ ⌜ False ⌝.
+  Proof.
+    iIntros "H1 H2". iDestruct (own_valid_2 with "H1 H2") as %Hv.
+    now apply excl_auth.excl_auth_frag_op_valid in Hv.
+  Qed.
+
+  Lemma program_update t t' :
+    program_auth t ∗ program_frag t ==∗
+    program_auth t' ∗ program_frag t'.
+  Proof.
+    rewrite /program_auth /program_frag. rewrite -!own_op.
+    iApply own_update. apply auth_update.
+    apply option_local_update.
+    apply exclusive_local_update. constructor.
+  Qed.
+
+  (* For the moment, there is no need for a lemma stating that traces can only be appened to, but we could customize the RA to enforce this. *)
+
+  #[export] Instance program_auth_Timeless t : Timeless (program_auth t).
+  Proof.
+    intros. apply _.
+  Qed.
+
+  #[export] Instance program_frag_Timeless t : Timeless (program_frag t).
+  Proof.
+    intros. apply _.
+  Qed.
+End S.
+
 (* invariants for memory, and a state interpretation for (mem,reg) *)
-Global Instance memG_irisG `{!memG Σ, !regG Σ} : irisGS asm_lang Σ := {
+Global Instance memG_irisG `{!memG Σ, !regG Σ, !traceG (list leak) Σ, !pcG Σ, !programG Σ} : irisGS asm_lang Σ := {
   iris_invGS := mem_invG;
-  state_interp σ _ κs _ := ((gen_heap_interp σ.1) ∗ (gen_heap_interp σ.2))%I;
+  state_interp σ _ κs _ := ((gen_heap_interp σ.1.2.1.2) ∗ (gen_heap_interp σ.1.2.2) ∗ tr_auth trace_name σ.2 ∗ pc_auth PC_name σ.1.2.1.1 ∗ program_auth Program_name σ.1.1)%I;
   fork_post _ := True%I;
   num_laters_per_step _ := 0;
   state_interp_mono _ _ _ _ := fupd_intro _ _
